rocq/Ender/CompleteChecker.v
@@ -1,0 +1,282 @@
+From Coq Require Import List String Bool.
+Require Import GeoCoq.Main.Tarski_dev.Ch11_angles.
+Require Import Ender.Audit Ender.PublicParser Ender.Syntax Ender.Semantics
+  Ender.Checker Ender.Parser.
+Import ListNotations.
+Import EnderSyntax.
+Module FA := Audit.FinalAudit.
+Open Scope string_scope.
+
+Definition project_segment (s : FA.SegmentName) : Segment :=
+  segment s.(FA.segment_first) s.(FA.segment_second).
+Definition project_angle (a : FA.AngleName) : Angle :=
+  angle a.(FA.angle_first) a.(FA.angle_vertex) a.(FA.angle_last).
+Definition project_triangle (t : FA.TriangleName) : Triangle :=
+  triangle t.(FA.triangle_first) t.(FA.triangle_second) t.(FA.triangle_third).
+
+(** Statements usable as premises by the currently implemented kernel. *)
+Definition project_premise_statement (s : FA.PublicStatement) : option Statement :=
+  match s with
+  | FA.ConSeg a b => Some (ConSeg (project_segment a) (project_segment b))
+  | FA.ConAng a b => Some (ConAng (project_angle a) (project_angle b))
+  | FA.RefSeg a b => Some (RefSeg (project_segment a) (project_segment b))
+  | FA.RefAng a b => Some (RefAng (project_angle a) (project_angle b))
+  | _ => None
+  end.
+
+(** Reflexive goals carry extra public same-object meaning not supplied merely
+    by internal congruence, so this adapter conservatively rejects them. *)
+Definition project_goal_statement (s : FA.PublicStatement) : option Statement :=
+  match s with
+  | FA.ConSeg a b => Some (ConSeg (project_segment a) (project_segment b))
+  | FA.ConAng a b => Some (ConAng (project_angle a) (project_angle b))
+  | FA.ConTri a b => Some (ConTri (project_triangle a) (project_triangle b))
+  | _ => None
+  end.
+
+Fixpoint project_premise_statements (ss : list FA.PublicStatement)
+    : option (list Statement) :=
+  match ss with
+  | [] => Some []
+  | s :: rest =>
+      match project_premise_statement s, project_premise_statements rest with
+      | Some x, Some xs => Some (x :: xs)
+      | _, _ => None
+      end
+  end.
+
+Definition projected_triangles (ds : list FA.PublicDeclaration) : list Triangle :=
+  fold_right (fun d rest => match d with
+    | FA.TriangleDeclaration t => project_triangle t :: rest
+    | _ => rest
+    end) [] ds.
+
+Fixpoint statement_list_eqb (a b : list Statement) : bool :=
+  match a, b with
+  | [], [] => true
+  | x :: xs, y :: ys => statement_eqb x y && statement_list_eqb xs ys
+  | _, _ => false
+  end.
+
+Fixpoint triangle_list_eqb (a b : list Triangle) : bool :=
+  match a, b with
+  | [], [] => true
+  | x :: xs, y :: ys => triangle_eqb x y && triangle_list_eqb xs ys
+  | _, _ => false
+  end.
+
+Definition premise_statements (ps : list Premise) : list Statement :=
+  map premise_statement ps.
+
+Definition goal_declarations_valid (goal : FA.PublicStatement)
+    (triangles : list Triangle) : bool :=
+  match goal with
+  | FA.ConTri a b => triangle_mem (project_triangle a) triangles &&
+                     triangle_mem (project_triangle b) triangles
+  | _ => true
+  end.
+
+Definition build_kernel_problem (public : FA.PublicProblem)
+    (header : ProblemHeader) (steps : list Step) : option Problem :=
+  match project_premise_statements public.(FA.public_premises),
+        project_goal_statement public.(FA.public_conclusion) with
+  | Some premises, Some goal =>
+      if triangle_list_eqb (projected_triangles public.(FA.public_declarations))
+                           header.(header_triangles) &&
+         statement_list_eqb premises (premise_statements header.(header_premises)) &&
+         statement_eqb goal header.(header_goal) &&
+         goal_declarations_valid public.(FA.public_conclusion)
+           header.(header_triangles)
+      then Some (problem header.(header_triangles) header.(header_premises) goal steps)
+      else None
+  | _, _ => None
+  end.
+
+Definition complete_checker (source : string) : bool :=
+  let text := list_ascii_of_string source in
+  match problemPart source,
+        Parser.find_after (list_ascii_of_string "steps:") text with
+  | Some part, Some stepText =>
+      match parsePublicProblem part, parseProblemPart part,
+            parse_step_lines (Parser.split_lines stepText []) [] with
+      | Some public, Some header, Some steps =>
+          match build_kernel_problem public header steps with
+          | Some p => check_problem p
+          | None => false
+          end
+      | _, _, _ => false
+      end
+  | _, _ => false
+  end.
+
+Lemma statement_list_eqb_eq : forall a b,
+  statement_list_eqb a b = true <-> a = b.
+Proof.
+  induction a as [|x xs IH]; destruct b as [|y ys]; cbn; try easy.
+  rewrite andb_true_iff, statement_eqb_eq, IH. split.
+  - intros [-> ->]. reflexivity.
+  - intros H. inversion H. auto.
+Qed.
+
+Lemma triangle_list_eqb_eq : forall a b,
+  triangle_list_eqb a b = true <-> a = b.
+Proof.
+  induction a as [|x xs IH]; destruct b as [|y ys]; cbn; try easy.
+  rewrite andb_true_iff, triangle_eqb_eq, IH. split.
+  - intros [-> ->]. reflexivity.
+  - intros H. inversion H. auto.
+Qed.
+
+Section Bridge.
+Context `{TnEQD : Tarski_neutral_dimensionless_with_decidable_point_equality}.
+Variable point : FA.PointName -> Tpoint.
+
+Lemma projected_triangle_meaning : forall declarations,
+  Forall (FA.declarationMeaning point) declarations ->
+  declarations_well_formed point (projected_triangles declarations).
+Proof.
+  intros declarations Hall t Hin. induction Hall as [|d ds Hd Hds IH]; cbn in Hin.
+  - contradiction.
+  - destruct d; cbn in *; try now apply IH.
+    destruct Hin as [<-|Hin]; [exact (proj2 (proj2 (proj2 Hd)))|now apply IH].
+Qed.
+
+Lemma projected_premise_meaning : forall public internal,
+  project_premise_statement public = Some internal ->
+  FA.statementMeaning point public -> interp_statement point internal.
+Proof.
+  destruct public; cbn; intros internal Hproject Hmeaning; try discriminate;
+    injection Hproject as <-; cbn in *; try exact Hmeaning; tauto.
+Qed.
+
+Lemma projected_premises_meaning : forall publics internals premises,
+  project_premise_statements publics = Some internals ->
+  premise_statements premises = internals ->
+  Forall (FA.statementMeaning point) publics ->
+  Forall (interp_premise point) premises.
+Proof.
+  intros publics. induction publics as [|s rest IH]; intros internals premises Hproject Heq Hall.
+  - cbn in Hproject. injection Hproject as <-. destruct premises; cbn in Heq;
+      [constructor|discriminate].
+  - cbn in Hproject. destruct (project_premise_statement s) as [x|] eqn:Hs;
+      try discriminate. destruct (project_premise_statements rest) as [xs|] eqn:Hrest;
+      try discriminate. injection Hproject as <-.
+    inversion Hall as [|? ? Hsmeaning Hrestmeaning]; subst.
+    destruct premises as [|p ps]; cbn in Heq; try discriminate.
+    injection Heq as Hhead Htail. constructor.
+    + unfold interp_premise. rewrite Hhead.
+      eapply projected_premise_meaning; eauto.
+    + eapply IH; eauto.
+Qed.
+
+Lemma noncol_well_formed : forall A B C,
+  ~ Col A B C -> A <> B /\ B <> C /\ C <> A /\ ~ Col A B C.
+Proof.
+  intros A B C H. pose proof (not_col_distincts A B C H) as Hd.
+  destruct Hd as [Hn [Hab [Hbc Hac]]]. repeat split; auto; congruence.
+Qed.
+
+Lemma projected_goal_meaning : forall public internal declarations,
+  project_goal_statement public = Some internal ->
+  interp_statement point internal ->
+  declarations_well_formed point declarations ->
+  goal_declarations_valid public declarations = true ->
+  FA.statementMeaning point public.
+Proof.
+  destruct public; cbn; intros internal declarations Hproject Hmeaning Hwf Hdecl;
+    try discriminate;
+    injection Hproject as <-; cbn in *; try exact Hmeaning.
+  apply andb_true_iff in Hdecl. destruct Hdecl as [Ha Hb].
+  apply triangle_mem_spec in Ha. apply triangle_mem_spec in Hb.
+  pose proof (Hwf _ Ha) as Hwa. pose proof (Hwf _ Hb) as Hwb.
+  apply noncol_well_formed in Hwa. apply noncol_well_formed in Hwb.
+  unfold triangle_congruence in Hmeaning. cbn in Hmeaning.
+  destruct Hmeaning as [Hab [Hbc [Hca Hangles]]].
+  unfold FA.TriangleCongruent. cbn.
+  exact (conj Hwa (conj Hwb (conj Hab (conj Hbc Hca)))).
+Qed.
+
+End Bridge.
+
+Theorem complete_checker_problem_sound : forall source part public,
+  problemPart source = Some part ->
+  parsePublicProblem part = Some public ->
+  complete_checker source = true ->
+  forall `{TnEQD : Tarski_neutral_dimensionless_with_decidable_point_equality},
+  forall point : FA.PointName -> Tpoint,
+    FA.problemClaim point public.
+Proof.
+  intros source part public Hpart Hpublic Hcheck Tn TnEQD point.
+  unfold complete_checker in Hcheck. rewrite Hpart, Hpublic in Hcheck.
+  destruct (Parser.find_after (list_ascii_of_string "steps:")
+              (list_ascii_of_string source)) as [stepText|] eqn:HstepText;
+    try discriminate.
+  destruct (parseProblemPart part) as [header|] eqn:Hheader; try discriminate.
+  destruct (parse_step_lines (Parser.split_lines stepText []) []) as [steps|]
+    eqn:Hsteps; try discriminate.
+  unfold build_kernel_problem in Hcheck.
+  destruct (project_premise_statements (FA.public_premises public)) as [premises|]
+    eqn:HprojectPremises; try discriminate.
+  destruct (project_goal_statement (FA.public_conclusion public)) as [goal|]
+    eqn:HprojectGoal; try discriminate.
+  destruct (triangle_list_eqb (projected_triangles (FA.public_declarations public))
+              (header_triangles header) &&
+            statement_list_eqb premises (premise_statements (header_premises header)) &&
+            statement_eqb goal (header_goal header) &&
+            goal_declarations_valid (FA.public_conclusion public)
+              (header_triangles header)) eqn:Hmatches; try discriminate.
+  apply andb_true_iff in Hmatches. destruct Hmatches as [Hrest HgoalDeclared].
+  apply andb_true_iff in Hrest. destruct Hrest as [Hrest Hgoal].
+  apply andb_true_iff in Hrest. destruct Hrest as [Htriangles Hpremises].
+  apply triangle_list_eqb_eq in Htriangles.
+  apply statement_list_eqb_eq in Hpremises.
+  apply statement_eqb_eq in Hgoal.
+  unfold FA.problemClaim. intros Hdeclarations HpublicPremises.
+  pose proof (projected_triangle_meaning point _ Hdeclarations) as Hwf.
+  rewrite Htriangles in Hwf.
+  assert (HkernelPremises :
+      Forall (interp_premise point) (header_premises header)).
+  { eapply projected_premises_meaning.
+    - exact HprojectPremises.
+    - symmetry. exact Hpremises.
+    - exact HpublicPremises. }
+  pose proof (check_problem_sound point
+    (problem (header_triangles header) (header_premises header) goal steps)
+    Hcheck Hwf HkernelPremises) as HkernelGoal.
+  eapply projected_goal_meaning; eauto.
+Qed.
+
+Module CompleteVerifiedChecker <: FA.COMPLETE_VERIFIED_CHECKER.
+  Definition parseProblem := parsePublicProblem.
+  Definition checker := complete_checker.
+  Definition parser_sound := parsePublicProblem_sound.
+
+  Definition meaning
+      `{TnEQD : Tarski_neutral_dimensionless_with_decidable_point_equality}
+      (source : string) : option Prop :=
+    match parseProblem source with
+    | Some p =>
+        Some (forall point : FA.PointName -> Tpoint, FA.problemClaim point p)
+    | None => None
+    end.
+
+  Theorem checker_sound : forall source,
+    checker source = true ->
+      forall part, problemPart source = Some part ->
+      forall `{TnEQD : Tarski_neutral_dimensionless_with_decidable_point_equality},
+      forall (T2D : @Tarski_2D Tn TnEQD),
+      forall (TE : @Tarski_euclidean Tn TnEQD),
+        exists claim : Prop, meaning part = Some claim /\ claim.
+  Proof.
+    intros source Hcheck part Hpart Tn TnEQD T2D TE.
+    unfold meaning, parseProblem.
+    destruct (parsePublicProblem part) as [public|] eqn:Hpublic.
+    - eexists. split; [reflexivity|].
+      intros point. exact (@complete_checker_problem_sound source part public
+        Hpart Hpublic Hcheck Tn TnEQD point).
+    - exfalso. unfold checker, complete_checker in Hcheck.
+      rewrite Hpart in Hcheck.
+      destruct (Parser.find_after (list_ascii_of_string "steps:")
+        (list_ascii_of_string source)); [rewrite Hpublic in Hcheck|]; discriminate.
+  Qed.
+End CompleteVerifiedChecker.
