rocq/Ender/Extract.v
@@ -1,5 +1,5 @@
 From Coq Require Import Extraction ExtrOcamlBasic ExtrOcamlString ExtrOcamlNatInt.
-Require Import Ender.Parser.
+Require Import Ender.CompleteChecker.
 
 Extraction Language OCaml.
-Extraction "extracted/EnderChecker.ml" check_source.
+Extraction "extracted/EnderChecker.ml" complete_checker.
